change state interp

dimsum/iris/sim.v
@@ -15,40 +15,41 @@ Class Sim (PROP : bi) (E1 E2 : Type) :=
 Notation "et '⪯{' E '}' es {{ Φ } }" := (sim E et es Φ) (at level 70, Φ at level 200,
   format "'[hv' et  '/' '⪯{' E '}'  '/' es  '/' {{  '[ ' Φ  ']' } } ']'") : bi_scope.
 
-Structure mod_lang EV := ModLang {
+Structure mod_lang Σ EV := ModLang {
   mexpr : Type;
   mtrans : mod_trans EV;
   mexpr_rel : mtrans.(m_state) → mexpr → Prop;
+  mstate_interp : mtrans.(m_state) → iProp Σ;
 }.
-Global Arguments mexpr {_} _.
-Global Arguments mtrans {_} _.
-Global Arguments mexpr_rel {_} _ _ _.
+Global Arguments mexpr {_ _} _.
+Global Arguments mtrans {_ _} _.
+Global Arguments mexpr_rel {_ _} _ _ _.
+Global Arguments mstate_interp {_ _} _ _.
 
-Definition mexprO {EV} {Λ : mod_lang EV} := leibnizO (mexpr Λ).
+Definition mexprO {Σ EV} {Λ : mod_lang Σ EV} := leibnizO (mexpr Λ).
 
 Class dimsumPreG (Σ : gFunctors) := RefirisPreG {
   dimsum_pre_invG :> invGpreS Σ;
   dimsum_pre_ord_laterG :> ord_laterPreG Σ;
 }.
 
-Class dimsumGS (EV : Type) (Λ_t Λ_s : mod_lang EV) (Σ : gFunctors) := DimsumGS {
+Class dimsumGS (EV : Type) (Σ : gFunctors) (Λ_t Λ_s : mod_lang Σ EV) := DimsumGS {
   dimsum_invGS :> invGS_gen HasNoLc Σ;
   dimsum_ord_laterGS :> ord_laterGS Σ;
-  state_interp : (mtrans Λ_t).(m_state) → (mtrans Λ_s).(m_state) → iProp Σ;
 }.
 Global Opaque dimsum_invGS.
 
-Definition sim_pre `{!dimsumGS EV Λ_t Λ_s Σ}
+Definition sim_pre `{!dimsumGS EV Σ Λ_t Λ_s}
     (sim : leibnizO coPset -d> mexprO -d> mexprO -d> (mexprO -d> mexprO -d> iPropO Σ) -d> iPropO Σ) :
     leibnizO coPset -d> mexprO -d> mexprO -d> (mexprO -d> mexprO -d> iPropO Σ) -d> iPropO Σ := λ E e_t e_s Φ,
   (∀ σ_t σ_s, ⌜mexpr_rel Λ_t σ_t e_t⌝ -∗ ⌜mexpr_rel Λ_s σ_s e_s⌝ -∗
-    ord_later_ctx -∗ state_interp σ_t σ_s ={E}=∗
-      (state_interp σ_t σ_s ∗ Φ e_t e_s) ∨
+    ord_later_ctx -∗ mstate_interp Λ_t σ_t -∗ mstate_interp Λ_s σ_s ={E}=∗
+      (mstate_interp Λ_t σ_t ∗ mstate_interp Λ_s σ_s ∗ Φ e_t e_s) ∨
       ∀ κ Pσ_t, ⌜(mtrans Λ_t).(m_step) σ_t κ Pσ_t⌝ ={E,∅}=∗ ▷ₒ
         ∃ Pσ_s, ⌜σ_s ~{mtrans Λ_s, option_trace κ}~>ₜ Pσ_s⌝ ∗
           ∀ σ_s', ⌜Pσ_s σ_s'⌝ ={∅, E}=∗
             ∃ σ_t' e_t' e_s', ⌜Pσ_t σ_t'⌝ ∗ ⌜mexpr_rel Λ_t σ_t' e_t'⌝ ∗ ⌜mexpr_rel Λ_s σ_s' e_s'⌝ ∗
-              (state_interp σ_t' σ_s' ∗ sim E e_t' e_s' Φ))%I.
+              (mstate_interp Λ_t σ_t' ∗ mstate_interp Λ_s σ_s' ∗ sim E e_t' e_s' Φ))%I.
 
 Global Instance sim_pre_ne `{!dimsumGS EV Λ_t Λ_s Σ} n:
   Proper ((dist n ==> dist n ==> dist n ==> dist n ==> dist n) ==> dist n ==> dist n ==> dist n ==> dist n ==> dist n) sim_pre.
@@ -62,15 +63,15 @@ Lemma sim_pre_mono `{!dimsumGS EV Λ_t Λ_s Σ} sim1 sim2:
   → ∀ E e_t e_s Φ , sim_pre sim1 E e_t e_s Φ -∗ sim_pre sim2 E e_t e_s Φ.
 Proof.
   iIntros "#Hinner" (E e_t e_s Φ) "Hsim".
-  iIntros (σ_t σ_s ??) "#? Hσ".
-  iMod ("Hsim" with "[//] [//] [//] Hσ") as "[Hsim|Hsim]"; [by iLeft|iRight]. iModIntro.
+  iIntros (σ_t σ_s ??) "#? Hσ_t Hσ_s".
+  iMod ("Hsim" with "[//] [//] [//] Hσ_t Hσ_s") as "[Hsim|Hsim]"; [by iLeft|iRight]. iModIntro.
   iIntros (κ P_tσ ?). iMod ("Hsim" with "[//]") as "Hsim". iModIntro. iMod "Hsim" as (??) "Hsim".
   iExists _. iSplit; [done|].
-  iIntros (??). iMod ("Hsim" with "[//]") as (??????) "[? ?]". iModIntro.
+  iIntros (??). iMod ("Hsim" with "[//]") as (??????) "[? [??]]". iModIntro.
   iSplit!; [done..|]. iFrame. by iApply "Hinner".
 Qed.
 
-Local Instance sim_pre_monotone `{!dimsumGS EV Λ_t Λ_s Σ} :
+Local Instance sim_pre_monotone `{!dimsumGS EV Σ Λ_t Λ_s} :
   BiMonoPred (λ sim : prodO (prodO (prodO (leibnizO coPset) mexprO) mexprO) (mexprO -d> mexprO -d> iPropO Σ) -d> iPropO Σ, uncurry4 (sim_pre (curry4 sim))).
 Proof.
   constructor.
@@ -80,17 +81,17 @@ Proof.
     apply sim_pre_ne; eauto. move => ???????????? /=. by apply: Hsim.
 Qed.
 
-Definition sim_def `{!dimsumGS EV Λ_t Λ_s Σ} : Sim (iPropI Σ) (mexpr Λ_t) (mexpr Λ_s) :=
+Definition sim_def `{!dimsumGS EV Σ Λ_t Λ_s} : Sim (iPropI Σ) (mexpr Λ_t) (mexpr Λ_s) :=
   curry4 (bi_least_fixpoint (λ sim : prodO (prodO (prodO (leibnizO coPset) mexprO) mexprO) (mexprO -d> mexprO -d> iPropO Σ) -d> iPropO Σ, uncurry4 (sim_pre (curry4 sim)))).
 Definition sim_aux : seal (@sim_def). Proof. by eexists. Qed.
 Definition sim' := sim_aux.(unseal).
-Global Arguments sim' {EV Λ_t Λ_s Σ _}.
+Global Arguments sim' {EV Σ Λ_t Λ_s _}.
 Global Existing Instance sim'.
-Lemma sim_eq `{!dimsumGS EV Λ_t Λ_s Σ} : sim = @sim_def EV Λ_t Λ_s Σ _.
+Lemma sim_eq `{!dimsumGS EV Σ Λ_t Λ_s} : sim = @sim_def EV Σ Λ_t Λ_s _.
 Proof. rewrite -sim_aux.(seal_eq) //. Qed.
 
 Section sim.
-Context `{!dimsumGS EV Λ_t Λ_s Σ}.
+Context `{!dimsumGS EV Σ Λ_t Λ_s}.
 Implicit Types s : stuckness.
 Implicit Types P : iProp Σ.
 Implicit Types Φ : mexpr Λ_t → mexpr Λ_s → iProp Σ.
@@ -123,7 +124,7 @@ Qed.
 
 Lemma sim_stop' E e_t e_s Φ:
   (|={E}=> Φ e_t e_s) -∗ e_t ⪯{E} e_s {{ Φ }}.
-Proof. rewrite sim_unfold. iIntros "HΦ" (σ_t σ_s ??) "? Hσ". iLeft. iFrame. Qed.
+Proof. rewrite sim_unfold. iIntros "HΦ" (σ_t σ_s ??) "? Hσ_t Hσ_s". iLeft. iFrame. Qed.
 Lemma sim_stop E e_t e_s Φ:
   Φ e_t e_s -∗ e_t ⪯{E} e_s {{ Φ }}.
 Proof. iIntros "HΦ". iApply sim_stop'. by iFrame. Qed.
@@ -131,16 +132,16 @@ Proof. iIntros "HΦ". iApply sim_stop'. by iFrame. Qed.
 
 Lemma sim_step E e_t e_s Φ:
   (∀ σ_t σ_s κ Pσ_t, ⌜mexpr_rel Λ_t σ_t e_t⌝ -∗ ⌜mexpr_rel Λ_s σ_s e_s⌝ -∗
-    ⌜(mtrans Λ_t).(m_step) σ_t κ Pσ_t⌝ -∗ state_interp σ_t σ_s ={E,∅}=∗ ▷ₒ
+    ⌜(mtrans Λ_t).(m_step) σ_t κ Pσ_t⌝ -∗ mstate_interp Λ_t σ_t -∗ mstate_interp Λ_s σ_s ={E,∅}=∗ ▷ₒ
       ∃ Pσ_s, ⌜σ_s ~{mtrans Λ_s, option_trace κ}~>ₜ Pσ_s⌝ ∗
          ∀ σ_s', ⌜Pσ_s σ_s'⌝ ={∅, E}=∗
            ∃ σ_t' e_t' e_s', ⌜Pσ_t σ_t'⌝ ∗ ⌜mexpr_rel Λ_t σ_t' e_t'⌝ ∗ ⌜mexpr_rel Λ_s σ_s' e_s'⌝ ∗
-              (state_interp σ_t' σ_s' ∗ e_t' ⪯{E} e_s' {{ Φ }})) -∗
+              (mstate_interp Λ_t σ_t' ∗ mstate_interp Λ_s σ_s' ∗ e_t' ⪯{E} e_s' {{ Φ }})) -∗
   e_t ⪯{E} e_s {{ Φ }}.
 Proof.
   iIntros "Hsim".
-  rewrite sim_unfold. iIntros (????) "#? Hσ !>". iRight. iIntros (???).
-  iMod ("Hsim" with "[//] [//] [//] [$]") as "Hsim". do 2 iModIntro.
+  rewrite sim_unfold. iIntros (????) "#? Hσ_t Hσ_s !>". iRight. iIntros (???).
+  iMod ("Hsim" with "[//] [//] [//] [$] [$]") as "Hsim". do 2 iModIntro.
   iDestruct "Hsim" as (??) "Hsim". iExists _. iSplit; [done|].
   iIntros (??). iMod ("Hsim" with "[//]") as (??????) "[? Hsim]".
   iModIntro. iSplit!; [done..|]. iFrame.
@@ -156,56 +157,66 @@ Proof.
   iIntros (?) "Hsim".
   iApply (sim_ind with "[] Hsim"). { solve_proper. }
   iIntros "!>" (????) "Hsim". iIntros (?) "Hc".
-  rewrite sim_unfold. iIntros (????) "#? Hσ".
-  iMod ("Hsim" with "[//] [//] [//] Hσ") as "[[? ?]|Hsim]".
-  - iDestruct ("Hc" with "[$]") as "Hc". rewrite sim_unfold. by iApply "Hc".
+  rewrite sim_unfold. iIntros (????) "#? Hσ_t Hσ_s".
+  iMod ("Hsim" with "[//] [//] [//] Hσ_t Hσ_s") as "[[? [??]]|Hsim]".
+  - iDestruct ("Hc" with "[$]") as "Hc". rewrite sim_unfold.
+    iApply ("Hc" with "[//] [//] [//] [$] [$]").
   - iModIntro. iRight. iIntros (???). iMod ("Hsim" with "[//]") as "Hsim". do 2 iModIntro.
     iDestruct "Hsim" as (??) "Hsim".
-    iExists _. iSplit; [done|]. iIntros (??). iMod ("Hsim" with "[//]") as (??????) "[? HF]". iModIntro.
+    iExists _. iSplit; [done|]. iIntros (??). iMod ("Hsim" with "[//]") as (??????) "[? [? HF]]". iModIntro.
     iSplit!; [done..|]. iFrame. by iApply "HF".
 Qed.
 
 (* TODO *)
-Definition sim_src (E : coPset) (κ : option EV) (e_s : mexpr Λ_s) (Φ : mexpr Λ_s → iProp Σ) :=
-  ∀ σ_t σ_s, ⌜mexpr_rel Λ_s σ_s e_s⌝ -∗ state_interp σ_t σ_s ={E,∅}=∗
-    ∃ Pσ_s, ⌜σ_s ~{mtrans Λ_s, option_trace κ}~>ₜ Pσ_s⌝ ∗
-       ∀ σ_s', ⌜Pσ_s σ_s'⌝ ={∅, E}=∗
-            ∃ e_s', ⌜mexpr_rel Λ_s σ_s' e_s'⌝ ∗
-              (state_interp σ_t σ_s' ∗ Φ e_s').
+(* Definition sim_src (E : coPset) (κ : option EV) (e_s : mexpr Λ_s) (Φ : mexpr Λ_s → iProp Σ) := *)
+(*   ∀ σ_t σ_s, ⌜mexpr_rel Λ_s σ_s e_s⌝ -∗ state_interp σ_t σ_s ={E,∅}=∗ *)
+(*     ∃ Pσ_s, ⌜σ_s ~{mtrans Λ_s, option_trace κ}~>ₜ Pσ_s⌝ ∗ *)
+(*        ∀ σ_s', ⌜Pσ_s σ_s'⌝ ={∅, E}=∗ *)
+(*             ∃ e_s', ⌜mexpr_rel Λ_s σ_s' e_s'⌝ ∗ *)
+(*               (state_interp σ_t σ_s' ∗ Φ e_s'). *)
 
 End sim.
 
-Theorem sim_adequacy Σ EV Λ_t Λ_s `{!dimsumPreG Σ} σ_t σ_s :
+Theorem sim_adequacy Σ EV `{!dimsumPreG Σ} m_t m_s :
   (∀ `{Hinv : !invGS_gen HasNoLc Σ} `{Hord : !ord_laterGS Σ},
-    ⊢ |={⊤}=> ∃ (stateI : (mtrans Λ_t).(m_state) → (mtrans Λ_s).(m_state) → iProp Σ),
-       let _ : dimsumGS EV Λ_t Λ_s Σ := DimsumGS _ _ _ _ _ _ stateI
+    ⊢ |={⊤}=>
+     ∃ (expr_t expr_s : Type),
+     ∃ (expr_rel_t : (m_trans m_t).(m_state) → expr_t → Prop),
+     ∃ (expr_rel_s : (m_trans m_s).(m_state) → expr_s → Prop),
+     ∃ (stateI_t : (m_trans m_t).(m_state) → iProp Σ),
+     ∃ (stateI_s : (m_trans m_s).(m_state) → iProp Σ),
+       let Λ_t := ModLang Σ EV expr_t (m_trans m_t) expr_rel_t stateI_t in
+       let Λ_s := ModLang Σ EV expr_s (m_trans m_s) expr_rel_s stateI_s in
+       let _ : dimsumGS EV Σ Λ_t Λ_s := DimsumGS _ _ _ _ _ _
        in
        ∃ e_t e_s,
-       ⌜mexpr_rel Λ_t σ_t e_t⌝ ∗ ⌜mexpr_rel Λ_s σ_s e_s⌝ ∗
-       stateI σ_t σ_s ∗
+       ⌜mexpr_rel Λ_t m_t.(m_init) e_t⌝ ∗ ⌜mexpr_rel Λ_s m_s.(m_init) e_s⌝ ∗
+       stateI_t m_t.(m_init) ∗ stateI_s m_s.(m_init) ∗
        e_t ⪯{⊤} e_s {{ λ _ _, |={⊤, ∅}=> False }}) →
-  trefines (Mod (mtrans Λ_t) σ_t) (Mod (mtrans Λ_s) σ_s).
+  trefines m_t m_s.
 Proof.
   intros Hsim. constructor => κs /thas_trace_n [n Htrace].
   apply (step_fupdN_soundness_no_lc _ 0 0) => ? /=. simpl in *. iIntros "_".
   iMod (ord_later_alloc n) as (?) "Ha". iDestruct (ord_later_ctx_alloc with "Ha") as "#?".
-  iMod Hsim as (stateI ?? Het Hes) "(Hσ & Hsim)". clear Hsim.
-  iInduction Htrace as [????? Hκs|???????? Hstep ?? Hlt Hκs|????????? Hκs Hle] "IH" forall (σ_s e_t e_s Het Hes).
+  iMod Hsim as "(%expr_t & %expr_s & % & % & %stateI_t & %stateI_s & % & % & %He_t & %He_s & Hσ_t & Hσ_s & Hsim)".
+  clear Hsim.
+  set (σ_t := m_init m_t) in *. set (σ_s := m_init m_s) in *. clearbody σ_t σ_s.
+  iInduction Htrace as [????? Hκs|???????? Hstep ?? Hlt Hκs|????????? Hκs Hle] "IH" forall (σ_s e_t e_s He_t He_s).
   - rewrite -Hκs. iApply fupd_mask_intro; [done|]. iIntros "HE". iPureIntro. by econstructor.
   - rewrite -Hκs. setoid_rewrite sim_unfold at 2.
-    iMod ("Hsim" with "[//] [//] [//] Hσ") as "[[? Hsim]|Hsim]". { by iMod "Hsim". }
-    iMod ("Hsim" with "[//]") as "Hsim".
+    iMod ("Hsim" with "[//] [//] [//] Hσ_t Hσ_s") as "[[? [? Hsim]]|Hsim]". { by iMod "Hsim". }
+    iMod ("Hsim" with "[//]") as "Hsim" => /=.
     iMod (ord_later_elim with "Hsim Ha [-]"); [|done]. iIntros "Ha".
     iMod (ord_later_update with "Ha"); [shelve|].
     iModIntro. iExists _. iFrame. iSplit; [done|]. iIntros "Ha".
     iDestruct 1 as (? Ht) "Hsim".
     iApply (fupd_mono _ _ ⌜_⌝). { iPureIntro. by apply thas_trace_trans. }
     iModIntro. iIntros (??).
-    iMod ("Hsim" with "[//]") as (σ_t' ???? ?) "[Hstate Hsim]".
+    iMod ("Hsim" with "[//]") as (σ_t' ???? ?) "[Hσ_t [Hσ_s Hsim]]".
     iMod (ord_later_update with "Ha") as "Ha"; [by apply: o_le_choice_r|].
-    iApply ("IH" with "[//] [//] Ha Hstate Hsim").
+    iApply ("IH" with "[//] [//] Ha Hσ_t Hσ_s Hsim").
     Unshelve. { by apply o_lt_impl_le. } { done. }
   - rewrite -Hκs. iApply (fupd_mono _ _ ⌜_⌝). { iPureIntro. apply thas_trace_all. }
     iIntros (?). iMod (ord_later_update with "Ha") as "Ha". { etrans; [|done]. by apply: o_le_choice_r. }
-    iApply ("IH" with "[//] [//] Ha Hσ Hsim").
+    iApply ("IH" with "[//] [//] Ha Hσ_t Hσ_s Hsim").
 Qed.
